MPPA - Added modulo and division 64 bits. Non certified
32 bits version are not yet there.

Right now the code is directly from libgcc, compiled with k1-gcc because
of builtins.

runtime/mppa_k1c/i64_sdiv.c
@@ -1,0 +1,29 @@
+unsigned long long
+udivmoddi4(unsigned long long num, unsigned long long den, int modwanted);
+
+long long
+__compcert_i64_sdiv (long long a, long long b)
+{
+  int neg = 0;
+  long long res;
+
+  if (a < 0)
+    {
+      a = -a;
+      neg = !neg;
+    }
+
+  if (b < 0)
+    {
+      b = -b;
+      neg = !neg;
+    }
+
+  res = udivmoddi4 (a, b, 0);
+
+  if (neg)
+    res = -res;
+
+  return res;
+}
+
