runtime/mppa_k1c/i64_smod.c
@@ -1,0 +1,25 @@
+unsigned long long
+udivmoddi4(unsigned long long num, unsigned long long den, int modwanted);
+
+long long
+__compcert_i64_smod (long long a, long long b)
+{
+  int neg = 0;
+  long long res;
+
+  if (a < 0)
+    {
+      a = -a;
+      neg = 1;
+    }
+
+  if (b < 0)
+    b = -b;
+
+  res = udivmoddi4 (a, b, 1);
+
+  if (neg)
+    res = -res;
+
+  return res;
+}
