runtime/mppa_k1c/i64_udivmod.c
@@ -1,0 +1,58 @@
+#ifdef __K1_TINYK1__
+unsigned long long
+udivmoddi4(unsigned long long num, unsigned long long den, int modwanted)
+{
+  unsigned long long bit = 1;
+  unsigned long long res = 0;
+
+  while (den < num && bit && !(den & (1L<<31)))
+    {
+      den <<=1;
+      bit <<=1;
+    }
+  while (bit)
+    {
+      if (num >= den)
+	{
+	  num -= den;
+	  res |= bit;
+	}
+      bit >>=1;
+      den >>=1;
+    }
+  if (modwanted) return num;
+  return res;
+}
+
+#else
+
+/* THIS IS THE PREVIOUS VERSION, USED ON BOSTAN AND ANDEY */
+unsigned long long
+udivmoddi4(unsigned long long num, unsigned long long den, int modwanted)
+{
+    unsigned long long r = num, q = 0;
+
+    if(den <= r) {
+	unsigned k = __builtin_clzll (den) - __builtin_clzll (r);
+	den = den << k;
+	if(r >= den) {
+	    r = r - den;
+	    q = 1LL << k;
+	}
+	if(k != 0) {
+	    unsigned i = k;
+	    den = den >> 1;
+	    do {
+		r = __builtin_k1_stsud (den, r);
+		i--;
+	    } while (i!= 0);
+	    q = q + r;
+	    r = r >> k;
+	    q = q - (r << k);
+	}
+    }
+
+    return modwanted ? r : q;
+}
+#endif	/* __K1_TINYK1__ */
+
