runtime/mppa_k1c/i64_umod.c
@@ -1,0 +1,9 @@
+unsigned long long
+udivmoddi4(unsigned long long num, unsigned long long den, int modwanted);
+
+unsigned long long
+__compcert_i64_umod (unsigned long long a, unsigned long long b)
+{
+  return udivmoddi4 (a, b, 1);
+}
+
