test/mppa/general/udivd.c
@@ -1,0 +1,8 @@
+#define TYPE unsigned long long
+
+int main(void){
+    TYPE a = 6;
+    TYPE b = -4;
+    
+    return a/b;
+}
